proof/correctness/avx2/mlkem_filters_bridge.ec
@@ -1,6 +1,8 @@
+timeout 1.
+
 require import AllCore List.
 from Jasmin require import JModel_x86.
-from JazzEC require import Array32 Array536 Array2048.
+from JazzEC require import Array32 Array48 Array24 Array536 Array2048.
 
 from CryptoSpecs require import Correctness.
 from JazzEC require import Jkem_avx2 (* Mlkem_filter48 *).
@@ -641,9 +643,9 @@ conseq  (bridge48 (to_uint _ctr) (to_uint _buf_offset) _pol)(filter48P (Array56.
   move => /= ? [# Hs1 Hs2] [# Hl1 Hl2] .
   split; last first. 
   + rewrite to_uint_eq Hs2 Hl2.
-    rewrite of_uintK /= modz_small. 
-  + rewrite /yy !size_map !size_filter /=; split; smt(@List take_oversize size_ge0 count_size size_filter size_bytes2coeffs W64.to_uint_cmp size_drop Array536.size_to_list).
-    smt(size_map).
+    rewrite of_uintK /= modz_small.
+  + rewrite /yy !size_map !size_filter /=; split; smt(@List size_map take_size take_oversize size_ge0 count_size size_filter size_bytes2coeffs W64.to_uint_cmp size_drop Array536.size_to_list).
+    by smt(size_map).
   + move :Hs1; rewrite Hl2.
     have ->: size xx = size yy by smt(size_map).
     move => ->.
@@ -662,7 +664,9 @@ conseq  (bridge48 (to_uint _ctr) (to_uint _buf_offset) _pol)(filter48P (Array56.
 (* THE MAIN LEMMA *)
 rewrite /yy /bytes2coeffs.
 have -> : BitEncoding.BitChunking.chunk 12 (JWordList.Bytes2Bits.bytes_to_bits (take 48 (drop (to_uint _buf_offset) (bufl _buf)))) =
-    map W12.w2bits (map (fun i => sliceget_8_12_56 ((init (fun (i0 : int) => _buf.[to_uint _buf_offset + i0])))%Array56 (12 * i)) (iota_ 0 32)); last first.
+    map W12.w2bits (map (fun i => sliceget_8_12_48
+                     (Array48.init ("_.[_]" (Array56.init (fun (i0 : int) => _buf.[to_uint _buf_offset + i0]))))
+                     (12 * i)) (iota_ 0 32)); last first.
 
 rewrite -map_comp -map_comp filter_map -map_comp.
 rewrite /xx pmap_map -map_comp filter_map -map_comp /(\o) /preim /=.
@@ -679,32 +683,48 @@ move => x l.
 pose F1 := (fun (x0 : int) =>
      to_uint
        (oget
-          (if sliceget_8_12_56 ((init (fun (i0 : int) => _buf.[to_uint _buf_offset + i0])))%Array56 (12 * x0) \ult
-              (W12.of_int 3329) then
-             Some (sliceget_8_12_56 ((init (fun (i0 : int) => _buf.[to_uint _buf_offset + i0])))%Array56 (12 * x0))
-           else None)%W12)).
+          (if sliceget_8_12_48
+                (Array48.init ("_.[_]" (Array56.init (fun (i0 : int) => _buf.[to_uint _buf_offset + i0]))))
+                (12 * x0) \ult
+              W12.of_int 3329 then
+             Some
+               (sliceget_8_12_48
+                  (Array48.init ("_.[_]" (Array56.init (fun (i0 : int) => _buf.[to_uint _buf_offset + i0]))))
+                  (12 * x0))
+           else None))).
 pose P1 := (fun (x0 : int) =>
         predC1 None
-          (if sliceget_8_12_56 ((init (fun (i0 : int) => _buf.[to_uint _buf_offset + i0])))%Array56 (12 * x0) \ult
-              (of_int 3329)%W12 then
-             Some (sliceget_8_12_56 ((init (fun (i0 : int) => _buf.[to_uint _buf_offset + i0])))%Array56 (12 * x0))
+          (if sliceget_8_12_48
+                (Array48.init ("_.[_]" (Array56.init (fun (i0 : int) => _buf.[to_uint _buf_offset + i0]))))
+                (12 * x0) \ult
+              W12.of_int 3329 then
+             Some
+               (sliceget_8_12_48
+                  (Array48.init ("_.[_]" (Array56.init (fun (i0 : int) => _buf.[to_uint _buf_offset + i0]))))
+                  (12 * x0))
            else None)).
 pose F2 := (fun (x0 : t) => to_uint ((of_int ((GFq.Zq.asint ((GFq.Zq.incoeff ((BitEncoding.BS2Int.bs2int (w2bits x0)))))))%GFq.Zq))%W16).
 pose P2 := (fun (x0 : t) => (BitEncoding.BS2Int.bs2int (w2bits x0)) < GFq.q).
 rewrite !filter_cons. 
 case (P1 x) => /=.
 + move => HP1 ->.
-  have HH /= : P2 (sliceget_8_12_56 ((init (fun (i0 : int) => _buf.[to_uint _buf_offset + i0])))%Array56 (12 * x)).
+  have HH /= : P2 (sliceget_8_12_48
+           (Array48.init ("_.[_]" (Array56.init (fun (i0 : int) => _buf.[to_uint _buf_offset + i0])))) (
+           12 * x)).
     + move : HP1; rewrite /P1 /P2 /=.
     by rewrite /predC1 ultE /= /to_uint /#.
   rewrite HH /F1 /F2.
    rewrite /predC1 ultE /= GFq.Zq.incoeffK /=.
-   pose a :=  (sliceget_8_12_56 ((init (fun (i0 : int) => _buf.[to_uint _buf_offset + i0])))%Array56 (12 * x)).
+   pose a :=  (sliceget_8_12_48
+              (Array48.init ("_.[_]" (Array56.init (fun (i0 : int) => _buf.[to_uint _buf_offset + i0]))))
+              (12 * x)).
   rewrite of_uintK /q /= modz_small 1:/# /to_uint /=.
   rewrite ifT 1:/# modz_small;smt(W12.to_uint_cmp).
 
 + move => HP1 ->.
-  have HH /= : !P2 (sliceget_8_12_56 ((init (fun (i0 : int) => _buf.[to_uint _buf_offset + i0])))%Array56 (12 * x)).
+  have HH /= : !P2 (sliceget_8_12_48
+           (Array48.init ("_.[_]" (Array56.init (fun (i0 : int) => _buf.[to_uint _buf_offset + i0])))) (
+           12 * x)).
     + move : HP1; rewrite /P1 /P2 /=.
     by rewrite /predC1 ultE /= /to_uint /#.
   rewrite /= HH /F1 /F2 => />.
@@ -738,7 +758,7 @@ size
 apply (eq_from_nth witness);1: smt(W12.size_w2bits). 
 rewrite Hs3;move => k kb.
 rewrite nth_take 1,2:/# nth_drop 1,2:/# /w2bits nth_mkseq 1:/# /=.
-rewrite /bytes_to_bits /sliceget_8_12_56 initiE 1:/# /= initiE 1:/# /=.
+rewrite /bytes_to_bits /sliceget_8_12_48 initiE 1:/# /= initiE 1:/#  initiE 1:/# /=.
 have -> := BitEncoding.BitChunking.nth_flatten witness 8 (map W8.w2bits (take 48 (drop (to_uint _buf_offset) (bufl _buf)))) (12*i+k) _.
 + rewrite allP => x.
   rewrite mapP => He; elim He => vv /=;smt(W8.size_w2bits).
@@ -1211,7 +1231,9 @@ conseq  (bridge24 (to_uint _ctr) (to_uint _buf_offset) _pol)(filter24P (Array32.
 (* THE MAIN LEMMA *)
 rewrite /yy /bytes2coeffs.
 have -> : BitEncoding.BitChunking.chunk 12 (JWordList.Bytes2Bits.bytes_to_bits (take 24 (drop (to_uint _buf_offset) (bufl _buf)))) =
-    map W12.w2bits (map (fun i => sliceget_8_12_32 ((init (fun (i0 : int) => _buf.[to_uint _buf_offset + i0])))%Array32 (12 * i)) (iota_ 0 16)); last first.
+    map W12.w2bits (map (fun i => sliceget_8_12_24
+                     (Array24.init ("_.[_]" (Array32.init (fun (i0 : int) => _buf.[to_uint _buf_offset + i0]))))
+                     (12 * i)) (iota_ 0 16)); last first.
 
 rewrite -map_comp -map_comp filter_map -map_comp.
 rewrite /xx pmap_map -map_comp filter_map -map_comp /(\o) /preim /=.
@@ -1228,32 +1250,46 @@ move => x l.
 pose F1 := (fun (x0 : int) =>
      to_uint
        (oget
-          (if sliceget_8_12_32 ((init (fun (i0 : int) => _buf.[to_uint _buf_offset + i0])))%Array32 (12 * x0) \ult
-              (W12.of_int 3329) then
-             Some (sliceget_8_12_32 ((init (fun (i0 : int) => _buf.[to_uint _buf_offset + i0])))%Array32 (12 * x0))
-           else None)%W12)).
+          (if sliceget_8_12_24
+                (Array24.init ("_.[_]" (Array32.init (fun (i0 : int) => _buf.[to_uint _buf_offset + i0])))) (
+                12 * x0) \ult
+              W12.of_int 3329 then
+             Some
+               (sliceget_8_12_24
+                  (Array24.init ("_.[_]" (Array32.init (fun (i0 : int) => _buf.[to_uint _buf_offset + i0])))) (
+                  12 * x0))
+           else None))).
 pose P1 := (fun (x0 : int) =>
         predC1 None
-          (if sliceget_8_12_32 ((init (fun (i0 : int) => _buf.[to_uint _buf_offset + i0])))%Array32 (12 * x0) \ult
-              (of_int 3329)%W12 then
-             Some (sliceget_8_12_32 ((init (fun (i0 : int) => _buf.[to_uint _buf_offset + i0])))%Array32 (12 * x0))
+          (if sliceget_8_12_24
+                (Array24.init ("_.[_]" (Array32.init (fun (i0 : int) => _buf.[to_uint _buf_offset + i0])))) (
+                12 * x0) \ult
+              W12.of_int 3329 then
+             Some
+               (sliceget_8_12_24
+                  (Array24.init ("_.[_]" (Array32.init (fun (i0 : int) => _buf.[to_uint _buf_offset + i0])))) (
+                  12 * x0))
            else None)).
 pose F2 := (fun (x0 : t) => to_uint ((of_int ((GFq.Zq.asint ((GFq.Zq.incoeff ((BitEncoding.BS2Int.bs2int (w2bits x0)))))))%GFq.Zq))%W16).
 pose P2 := (fun (x0 : t) => (BitEncoding.BS2Int.bs2int (w2bits x0)) < GFq.q).
 rewrite !filter_cons. 
 case (P1 x) => /=.
 + move => HP1 ->.
-  have HH /= : P2 (sliceget_8_12_32 ((init (fun (i0 : int) => _buf.[to_uint _buf_offset + i0])))%Array32 (12 * x)).
+  have HH /= : P2 (sliceget_8_12_24 (Array24.init ("_.[_]" (Array32.init (fun (i0 : int) => _buf.[to_uint _buf_offset + i0]))))
+           (12 * x)).
     + move : HP1; rewrite /P1 /P2 /=.
     by rewrite /predC1 ultE /= /to_uint /#.
   rewrite HH /F1 /F2.
    rewrite /predC1 ultE /= GFq.Zq.incoeffK /=.
-   pose a :=  (sliceget_8_12_32 ((init (fun (i0 : int) => _buf.[to_uint _buf_offset + i0])))%Array32 (12 * x)).
+   pose a :=  (sliceget_8_12_24
+              (Array24.init ("_.[_]" (Array32.init (fun (i0 : int) => _buf.[to_uint _buf_offset + i0])))) (
+              12 * x)).
   rewrite of_uintK /q /= modz_small 1:/# /to_uint /=.
   rewrite ifT 1:/# modz_small;smt(W12.to_uint_cmp).
 
 + move => HP1 ->.
-  have HH /= : !P2 (sliceget_8_12_32 ((init (fun (i0 : int) => _buf.[to_uint _buf_offset + i0])))%Array32 (12 * x)).
+  have HH /= : !P2 (sliceget_8_12_24 (Array24.init ("_.[_]" (Array32.init (fun (i0 : int) => _buf.[to_uint _buf_offset + i0]))))
+           (12 * x)).
     + move : HP1; rewrite /P1 /P2 /=.
     by rewrite /predC1 ultE /= /to_uint /#.
   rewrite /= HH /F1 /F2 => />.
@@ -1287,7 +1323,7 @@ size
 apply (eq_from_nth witness);1: smt(W12.size_w2bits). 
 rewrite Hs3;move => k kb.
 rewrite nth_take 1,2:/# nth_drop 1,2:/# /w2bits nth_mkseq 1:/# /=.
-rewrite /bytes_to_bits /sliceget_8_12_32 initiE 1:/# /= initiE 1:/# /=.
+rewrite /bytes_to_bits /sliceget_8_12_32 initiE 1:/# /= initiE 1:/# initiE 1:/# /=.
 have -> := BitEncoding.BitChunking.nth_flatten witness 8 (map W8.w2bits (take 24 (drop (to_uint _buf_offset) (bufl _buf)))) (12*i+k) _.
 + rewrite allP => x.
   rewrite mapP => He; elim He => vv /=;smt(W8.size_w2bits).
